thy/IDP_Report/Chap_Implementation.thy
@@ -1,0 +1,29 @@
+(*<*)
+theory Chap_Implementation
+imports Main
+begin
+(*>*)
+
+chapter\<open>Implementation\<close>
+section\<open>Overview\<close>
+text\<open>The sections of this chapter describe the different aspects of the implementation and present the most important theorems on them.\<close>
+
+text\<open>The (sub-)sections are presented in the topological order of the dependencies of the underlying theory code.
+We chose this order because it allows us to only introduce a definition when we have introduced all the things it is based on.
+Unfortunately, this means that it cannot always be clear why a definition has been made in a certain way,
+as the purpose of its details are often only revealed upon use.
+\<close>
+text\<open>Section \ref{sec:routing} shows a formalization of routing tables 
+and documents tools for parsing, analyzing and transforming routing tables.\<close>
+text\<open>Based upon that, \ref{sec:rpf} shows a formalization of Reverse Path Filtering.
+The main results presented there are a hierarchy of the different reverse path filtering types and a 
+transformation of routing tables to mappings for reverse path filtering.\<close>
+text\<open>The goal of sections \ref{sec:routing,sec:rpf} is to produce a relation that describes 
+the relation between interfaces and what set of IP addresses are allowed or expected to appear on these interfaces.\<close>
+text\<open>Based upon that and \todo{cite}, Section \ref{sec:irew} shows a method to refine the analysis of firewall rulesets
+by transforming interface matches to matches on IP addresses.\<close>
+
+
+(*<*)
+end
+(*>*)
