thy/IDP_Report/EvalLOFT.thy
@@ -1,0 +1,11 @@
+(*<*)
+theory EvalLOFT
+imports Main
+begin
+(*>*)
+
+section\<open>Re-evaluation of LOFT\<close>
+
+(*<*)
+end
+(*>*)
