thy/IDP_Report/RPF.thy
@@ -1,0 +1,185 @@
+(*<*)
+theory RPF
+imports  "../Routing/ReversePathFiltering" Routing
+begin
+(*>*)
+
+section\<open>Reverse Path Forwarding\<close>
+text_raw\<open>\label{sec:rpf}\<close>
+text\<open>Note: This section does not bear any significance for further sections, it is ``merely'' an interesting consideration.\<close>
+text\<open>In Section \ref{sec:routing_ipass}, we introduced the IP assignment as a relation
+that describes which destination IP addresses can be forwarded to which ports.
+Among other things, this section explores IP assignments as the converse:
+as a relation that describes which source IP addresses are expected to arrive on which interfaces%
+\footnote{Historically, we actually used IP assignments for this first.
+The explanation flows smoother in this order.}.
+\<close>
+text\<open>While source address spoofing takes away any possible way to know
+what source addresses can be expected for traffic arriving at interfaces,
+there are techniques to discard traffic with source addresses that can immediately be recognized as spoofed
+(i.e., recognize traffic tolerating false accepts but trying to avoid false rejects).
+These techniques are collected in RFC3704: ``Ingress Filtering for Multihomed Networks''.
+Since they are derived from the homonymous techniques for avoiding loops when forwarding multicast traffic\todo{cite?},
+they are more commonly known as \emph{Reverse Path Forwarding}%
+\footnote{Sometimes erroneously named ``Reverse Path Filtering''.} (RPF).
+The information that is necessary for RPF comes from the Forwarding Information Base (FIB).
+If we reuse the assumptions we made in Section \ref{sec:realrouting},
+the only thing that is relevant is thus the routing table.
+We made all definitions of this section based on that assumption.\<close>
+
+text\<open>RFC 3704 defines five ways of implementing RPF:
+\begin{itemize}
+  \item Ingress Access Lists
+  \item Strict Reverse Path Forwarding
+    \begin{quote}``The procedure is that the
+     source address is looked up in the FIB
+     — and if the packet is received on the interface which would be used
+     to forward the traffic to the source of the packet, it passes the
+     check.''\end{quote}
+  \item Feasible Path Reverse Path Forwarding
+    \begin{quote}
+      ``The source address is still looked up in the FIB (or
+      an equivalent, RPF-specific table) but instead of just inserting one
+      best route there, the alternative paths (if any) have been added as
+      well, and are valid for consideration.''
+    \end{quote}
+  \item Loose Reverse Path Forwarding
+    \begin{quote}
+      ``It checks only for the existence of a route (even a default route, if applicable), not where the route points to.''
+    \end{quote}
+  \item Loose Reverse Path Forwarding ignoring default routes
+    \begin{quote}
+    ``In the lookup, default routes are excluded.''
+    \end{quote}
+    (note that there are some variants defined in the RFC.)
+\end{itemize}
+The first item, Ingress Access Lists, just means to specify a list of acceptable source addresses for each interface.
+In other words, it requires the user to statically specify the source IP assignment.
+As such, it is of not much further interest \emph{inside} this section since its behavior can not be derived from the routing table.
+The rest of the section is going to continue with the four remaining types.
+They can be formalized in the following ways:
+\<close>
+lemma "rpf_strict rtbl p \<equiv> case routing_table_semantics rtbl (p_src p) of
+  Some ra \<Rightarrow> output_iface ra = p_iiface p | 
+  None \<Rightarrow> False" using rpf_strict_def .
+lemma "rpf_feasible rtbl p \<equiv> \<exists>rr \<in> set rtbl.
+  prefix_match_semantics (routing_match rr) (p_src p) \<and> routing_oiface rr = p_iiface p"
+  using rpf_feasible_def .
+lemma "rpf_loose rtbl p \<equiv> \<exists>rr \<in> set rtbl. prefix_match_semantics (routing_match rr) (p_src p)"
+  using rpf_loose_def .
+lemma "rpf_loose_ign_default rtbl p \<equiv> \<exists>rr \<in> set rtbl. 
+  prefix_match_semantics (routing_match rr) (p_src p) \<and> routing_match rr \<noteq> PrefixMatch 0 0"
+  using rpf_loose_ign_default_def .
+
+text\<open>At this point, one might ask whether the above 4 definitions are all sensible ways
+  to derive a decision for the source address from the routing table.
+  As RFC 3704 already answers this question negatively, here is an example of how one might formalize another level.\<close>
+lemma "rpf_semifeasible rtbl p \<equiv> \<exists>rr \<in> set rtbl. 
+   prefix_match_semantics (routing_match rr) (p_src p) \<and> routing_oiface rr = p_iiface p
+\<and> (\<forall>ra \<in> set rtbl. routing_prefix ra > routing_prefix rr \<longrightarrow>  \<not>prefix_match_semantics (routing_match ra) (p_src p))"
+  using rpf_semifeasible_def .
+text\<open>This definition is in the middle of strict and feasible RPF:
+It allows alternate routes, but only if the alternate routes have the same prefix length.
+(This might be useful when using a routing table that has been obtained from a routing protocol
+before doing link aggregation\todo{what can I cite?}. However, the reason we show it is its apparent similarity to
+@{const longest_prefix_routing}.)
+The general answer is (we did not verify this) that there is an infinite amount of possible definitions for RPF based on routing tables
+(and these can actually be put into an infinite hierarchy).
+We will thus not indulge in any further definitions of RPFs and concentrate on the ones we have.
+\<close>
+subsection\<open>A hierarchy\<close>
+text\<open>One interesting question is whether those definitions stand in any proper relation to each other.
+This question is positively answered for all but @{const rpf_loose_ign_default} by Figure \ref{fig:rpfhierar}.
+If there is an implication between two of the definitions,
+packets that are accepted by the antecedent are also accepted by the succedent.
+(All implications have been verified, but they are of the form @{thm rpf_feasible_loose[no_vars]} 
+and we decided not to state them all explicitly.
+The only exception is the implication from @{const rpf_strict} to @{const rpf_semifeasible},
+which also requires three of the routing table validity criteria: @{thm rpf_strict_semifeasible[no_vars]}.
+\<close>
+text_raw\<open>
+\begin{figure}
+\centering
+\begin{tikzpicture}[
+  dli/.style={
+    %->,
+    %postaction={overlay,double,draw,thick}
+    -implies,
+    double equal sign distance
+  }
+]
+\node (s) {@{const rpf_strict}};
+\node[below=of s] (sf) {@{const rpf_semifeasible}};
+\node[below=of sf] (f) {@{const rpf_feasible}};
+\node[below=of f] (l) {@{const rpf_loose}};
+\node[right=of l] (lid) {@{const rpf_loose_ign_default}};
+\draw[dli] (s) -- (sf);
+\draw[dli] (sf) -- (f);
+\draw[dli] (f) -- (l);
+\draw[dli] (lid) -- (l);
+\draw[dli,dashed] (lid) edge[bend right=20,->] (s);
+\draw[dli,dashed] (l) edge[bend left=50,->] (lid);
+\end{tikzpicture}
+\caption{The hierarchy of RPF implementations.}
+The dashed implications depend on the routing table.
+\label{fig:rpfhierar}
+\end{figure}
+\<close>
+text\<open>Interestingly, it is possible to find routing tables that fulfil all validity criteria%
+\footnote{@{thm all_valid_rtbl_def[no_vars]}} and make @{const rpf_loose_ign_default} deny any packet, 
+while @{const rpf_strict} still accepts some packets (the trick is to only have default routes).
+On the other hand side, it is also possible to find routing tables
+that make @{const rpf_loose} and @{const rpf_loose_ign_default} behave completely equal
+(the trick is to shadow any default rule completely).\<close>
+lemma 
+  "\<exists>rtbl. all_valid_rtbl rtbl \<and> (\<forall>p. \<not>rpf_loose_ign_default rtbl p) \<and> (\<exists>p. rpf_strict rtbl p)"
+  "\<exists>rtbl :: 32 prefix_routing. all_valid_rtbl rtbl \<and> (\<forall>p. rpf_loose rtbl p \<longleftrightarrow> rpf_loose_ign_default rtbl p)"
+  using ign_default_mean1 ign_default_mean2 by blast+
+
+subsection\<open>Obtaining IP assignments\<close>
+text\<open>Having learned all these things, it is time to answer the central question of this section:
+Can appropriate (source) IP assignments be derived from routing tables for all the different RPF types?
+For string RPF, this question is immediately answered by @{const routing_ipassmt_wi} from Section \ref{sec:routing_ipass} – the assignment is fully equal.
+For all other types, special definitions are necessary, and the two variants of loose RPF need an additional list of possible source interfaces.
+Since the actual definitions are not very insightful, we have collected them in @{const rpf_wi_lookup} and just show the following:
+\<close>
+theorem "\<lbrakk>valid_prefixes rtbl; rpf_type \<in> {RPF_Loose, RPF_LooseIgnDef} \<Longrightarrow> p_iiface p \<in> set ifs\<rbrakk>
+\<Longrightarrow> rpf_def_lookup rpf_type rtbl p = (\<exists>(k, l)\<in>set (rpf_wi_lookup rpf_type ifs rtbl). 
+  p_iiface p = k \<and> p_src p \<in> wordinterval_to_set l)" using rpf_ipassms .
+text\<open>where\<close>
+lemma "rpf_def_lookup rpf_type \<in> {rpf_strict, rpf_feasible, rpf_loose, rpf_loose_ign_default, rpf_semifeasible}"
+  by(rule rpf_type.exhaust[of rpf_type]; simp) (* interesting way to do a case distinction *)
+
+text\<open>Finally, it is time to evaluate whether all the definitions we have made here are worth anything. 
+The first thing that should strike us is the fact that one of the validity criteria we requested of a routing table 
+is that it contains a default route.
+If we require that and test @{const rpf_loose}, we immediately see that it accepts all packets.\<close>
+lemma "valid_prefixes rtbl \<Longrightarrow> has_default_route rtbl \<Longrightarrow> \<forall>p. rpf_loose rtbl p"
+  using default_loose_all .
+text\<open>
+The RFC 3704 authors must have realized this and authored the following paragraph:
+\begin{quote}
+  The questionable benefit of Loose RPF is found in asymmetric routing
+   situations: a packet is dropped if there is no route at all, such as
+   to "Martian addresses" or addresses that are not currently routed,
+   but is not dropped if a route exists.
+\end{quote}
+These aspects have fallen prey to our model of routing,
+degrading loose RPF from having a ``questionable benefit'' to being entirely useless.
+\<close>
+text\<open>Furthermore, we know from testing experience that
+we want at least an entry for the loopback interface in any source IP assignment.
+Unfortunately, the routing rule taking care or the local delivery of \texttt{127.0.0.0/8}
+is in the \texttt{local} table and will thus not be considered by our model.\<close>
+
+text\<open>In the end, we decided that the theoretical foundation of using RPF
+to obtain source IP assignments from routing tables is still a bit too weak
+to activate it as an available algorithm in an automated checking tool.
+Instead, we deferred to having the user provide a source IP assignment.
+In a sense, we will be using Ingress Access Lists.
+\<close>
+
+
+(*<*)
+end
+(*>*)
